Db/Migration/Basic.lean
@@ -4,8 +4,94 @@ import Db.Utils.Equiv
 structure Indexing.Map {α β : Type} [Indexing α] [Indexing β] (f : α → β) : Prop where
   toString_apply (a : α) : ToString.toString (f a) = ToString.toString a
 
+structure Indexing.Equiv (α β : Type) [Indexing α] [Indexing β] extends α ≃ β where
+  indexing_toFun : Indexing.Map toFun
+
+@[ext]
+def Indexing.Equiv.ext {α β : Type} [Indexing α] [Indexing β]
+    {e₁ e₂ : Indexing.Equiv α β} (h : e₁.toFun = e₂.toFun) :
+    e₁ = e₂ := by
+  cases e₁
+  cases e₂
+  simp only [mk.injEq]
+  ext1
+  exact h
+
+@[simp]
+theorem Indexing.Equiv.toString_toFun {α β : Type} [Indexing α] [Indexing β]
+    (e : Indexing.Equiv α β) (a : α) :
+    ToString.toString (e.toFun a) = ToString.toString a :=
+  e.indexing_toFun.toString_apply _
+
+@[simp]
+theorem Indexing.Equiv.toString_invFun {α β : Type} [Indexing α] [Indexing β]
+    (e : Indexing.Equiv α β) (b : β) :
+    ToString.toString (e.invFun b) = ToString.toString b := by
+  rw [← e.toFun_invFun b, toString_toFun, e.toFun_invFun]
+
+section
+
+variable (α β : Type) [Indexing α] [Indexing β]
+
+instance (α β : Type) [Indexing α] [Indexing β] : Subsingleton (Indexing.Equiv α β) where
+  allEq x y := by
+    ext a
+    apply Indexing.injective_toString
+    simp
+
+-- TODO: this is currently wrong, because we ask nothing for `Enum.all`
+theorem Indexing.Equiv.nonempty_iff :
+    Nonempty (Indexing.Equiv α β) ↔
+      ((Enum.all α).toList.map ToString.toString).Perm
+        ((Enum.all β).toList.map ToString.toString) := by
+  sorry
+
+instance : Decidable (Nonempty (Indexing.Equiv α β)) :=
+  decidable_of_decidable_of_iff (Indexing.Equiv.nonempty_iff _ _).symm
+
+end
+
 structure Table.Migration (source target : Table) where
-  map : source.Index → target.Index
+  map : source.Index → Option target.Index
+
+inductive Table.MigrationStep' (source target : Table) where
+  | dropColumn (index : source.Index)
+  | addColumn (index : target.Index)
+  | alterColumn (old : source.Index) (new : target.Index)
+
+def Table.Migration.steps {source target : Table} (migration : source.Migration target) :
+    List (source.MigrationStep' target) := Id.run <| do
+  let mut ops := []
+  let mut visited : Std.HashSet target.Index := .emptyWithCapacity
+  for index in Enum.all source.Index do
+    match migration.map index with
+    | some val =>
+      visited := visited.insert val
+      ops := .alterColumn index val :: ops
+    | none => ops := .dropColumn index :: ops
+  for index in Enum.all target.Index do
+    if index ∈ visited then
+      continue
+    ops := .addColumn index :: ops
+  return ops
+
+def Table.columnOfString (table : Table) (s : String) : Option Column := do
+  return table.columns (← FromString.fromString s)
+
+def Table.Equivalent (source target : Table) : Prop :=
+  ∃ (e : Indexing.Equiv source.Index target.Index),
+    ∀ i, target.columns (e.toFun i) = source.columns i
+
+theorem Table.Equivalent.iff (source target : Table) :
+    source.Equivalent target ↔
+      Nonempty (Indexing.Equiv source.Index target.Index) ∧
+        (Enum.all source.Index).all fun idx ↦
+          source.columnOfString (ToString.toString idx) ==
+            target.columnOfString (ToString.toString idx) :=
+  sorry
+
+instance (source target : Table) : Decidable (Table.Equivalent source target) :=
+  decidable_of_decidable_of_iff (Table.Equivalent.iff source target).symm
 
 /--
 A migration from database stage `source` to database stage `target`
