Db/Utils/Enum.lean
@@ -1,9 +1,135 @@
+import Lean
+import Db.Utils.Equiv
+import Db.Utils.FinCases
 import Std
+import Qq
 
-universe u
+universe u' u
 
-class Enum (α : Type u) : Type u extends Hashable α where
-  [decidableEq : DecidableEq α]
-  all (α) : Std.HashSet α
+class Enum (α : Type u) where
+  length (α) : Nat
+  encoding : α ≃ (Fin length)
 
-attribute [instance] Enum.decidableEq
+instance (n : Nat) : Enum (Fin n) where
+  length := n
+  encoding := .refl _
+
+def Enum.all (α : Type u) [Enum α] : Array α :=
+  .ofFn Enum.encoding.invFun
+
+def Fin.distribM {m : Type u → Type u'} [Monad m] {n : Nat} {α : Fin n → Type u}
+    (f : (i : Fin n) → m (α i)) : m ((i : Fin n) → α i) :=
+  match n with
+  | 0 => pure fun i => False.elim (by grind [i.2])
+  | n + 1 => do
+    let g : (i : Fin n) → α ⟨i.1, by grind⟩ ←
+      distribM fun j => f ⟨j.1, by grind⟩
+    let x ← f (.last n)
+    return fun j =>
+      if hj : j < n
+        then
+          g ⟨j, by grind⟩
+        else
+          cast (congrArg _ <| by grind) x
+
+def Enum.distribM {α : Type u} [Enum α] {m : Type u → Type u'} [Monad m] {β : α → Type u}
+    (f : (a : α) → m (β a)) :
+    m ((a : α) → β a) := do
+  let g ← Fin.distribM fun i => f <| Enum.encoding.invFun i
+  return fun a => cast (congrArg _ <| by simp) <| g (Enum.encoding.toFun a)
+
+open Qq Lean Elab Command
+
+def fromEnumWithMotive (name : Name) (expr : Array Expr) (motive : Expr) : MetaM Expr := do
+  Meta.withLocalDecl `x BinderInfo.default (.const name []) fun x => do
+    let body ← Meta.mkAppOptM (name ++ `casesOn) (#[some motive, some x] ++ (expr.map Option.some))
+    Meta.mkLambdaFVars #[x] body
+
+def fromEnum (name : Name) (expr : Array Expr) (type : Expr) : MetaM Expr := do
+  let motive : Expr ← Meta.withLocalDecl `x BinderInfo.default (.const name []) fun x => do
+    Meta.mkLambdaFVars #[x] type
+  fromEnumWithMotive name expr motive
+
+def Lean.Expr.getForallArgs : Expr → List (Name × Expr)
+  | .forallE n t b _ => (n, t) :: getForallArgs b
+  | _ => []
+
+def getStructureArgs {m : Type → Type} [Monad m] [MonadEnv m] [MonadError m] (decl : Name) :
+    m (List (Name × Expr)) := do
+  let .inductInfo info := ← getConstInfo decl | throwError "Not a structure."
+  unless info.ctors.length == 1 do throwError "Not a structure."
+  let ctor := info.ctors[0]!
+  let ctorInfo ← getConstInfo ctor
+  return ctorInfo.type.getForallArgs
+
+def Fin.asExpr {n : Nat} (i : Fin n) : Expr :=
+  q($i)
+
+def List.asExpr (type : Expr) : List Expr → MetaM Expr
+  | [] => Meta.mkAppOptM ``List.nil #[type]
+  | x :: xs => do Meta.mkAppM ``List.cons #[x, ← xs.asExpr type]
+
+def elabInstance (expr : Expr) : CommandElabM Unit := do
+  let instName : Name ← Lean.mkAuxDeclName
+  let instDecl : Declaration := .defnDecl
+    { name := instName
+      levelParams := []
+      type := ← liftTermElabM <| Meta.inferType expr
+      value := expr
+      hints := default
+      safety := .safe }
+  liftCoreM <| addAndCompile instDecl
+  liftTermElabM <| Meta.addInstance instName default 1000
+
+def deriveEnum (declNames : Array Name) : CommandElabM Bool := do
+  unless declNames.size = 1 do return false
+  let decl := declNames[0]!
+  let .inductInfo info := ← getConstInfo decl | throwError "Not a structure."
+  let fields : List Name := info.ctors
+  let fieldsWithIdx : List (Name × Fin fields.length) :=
+    fields.zip (List.finRange fields.length)
+  let enum : Expr ← liftTermElabM <| do
+    let length : Expr := .lit <| .natVal fields.length
+    let finType : Expr ← Meta.mkAppM ``Fin #[length]
+    let equiv : Expr ← do
+      let toFun : Expr ←
+        fromEnum declNames[0]!
+          (fieldsWithIdx.toArray.map fun f => f.2.asExpr)
+          finType
+      let invFun : Expr ← Meta.withLocalDecl `x BinderInfo.default finType fun x => do
+        let listExpr : Expr ←
+          List.asExpr (.const declNames[0]! []) (fields.map fun x => .const (x) [])
+        let body ← Meta.mkAppM ``List.get #[listExpr, x]
+        Meta.mkLambdaFVars #[x] body
+      let appEquiv ← Meta.mkAppOptM ``Equiv.mk #[Expr.const declNames[0]! [], finType, toFun, invFun]
+      match (← Meta.inferType appEquiv).getForallArgs with
+      | [(_name₁, type₁), (_name₂, type₂)] =>
+        let e₁ ← Meta.mkFreshExprMVar type₁
+        _ ← Elab.runTactic e₁.mvarId!
+          (← `(tactic| intro x; induction x <;> rfl))
+        let e₂ ← Meta.mkFreshExprMVar type₂
+        _ ← Elab.runTactic e₂.mvarId!
+          (← `(tactic| intro i; fincases i <;> rfl))
+        Meta.mkAppM' appEquiv #[e₁, e₂]
+      | _ => throwError "Failed when constructing `Enum` instance."
+    Meta.mkAppM ``Enum.mk #[length, equiv]
+  elabInstance enum
+  return true
+
+initialize registerDerivingHandler ``Enum deriveEnum
+
+section Test
+
+elab "derive_enum" name:ident : command => do
+  _ ← deriveEnum #[name.getId]
+
+inductive Baboosh
+  | a
+  | b
+  | c
+
+derive_enum Baboosh
+
+example : Enum.encoding.invFun 1 = Baboosh.b := rfl
+
+end Test
