Db/Utils/Equiv.lean
@@ -1,15 +1,44 @@
-universe u v
+universe u₁ u₂ u₃ u₄ u v
 
 structure Equiv (α : Type u) (β : Type v) where
   toFun : α → β
   invFun : β → α
-  invFun_toFun (a : α) : invFun (toFun a) = a
-  toFun_invFun (b : β) : toFun (invFun b) = b
+  invFun_toFun (a : α) : invFun (toFun a) = a := by grind
+  toFun_invFun (b : β) : toFun (invFun b) = b := by grind
+
+attribute [simp, grind =] Equiv.invFun_toFun Equiv.toFun_invFun
 
 notation α:max " ≃ " β:max => Equiv α β
+
+@[ext]
+theorem Equiv.ext {α : Type u} {β : Type v} {e₁ e₂ : α ≃ β}
+    (h : e₁.toFun = e₂.toFun) : e₁ = e₂ := by
+  obtain ⟨toFun₁, invFun₁, h₁₁, h₁₂⟩ := e₁
+  obtain ⟨toFun₂, invFun₂, h₂₁, h₂₂⟩ := e₂
+  simp only [mk.injEq]
+  refine ⟨h, ?_⟩
+  ext b
+  dsimp at h
+  rw [← h₂₂ b, h₂₁, ← h, h₁₁]
 
 def Equiv.refl (α : Type u) : α ≃ α where
   toFun := id
   invFun := id
-  invFun_toFun := by grind
-  toFun_invFun := by grind
+
+def Equiv.trans {α : Type u₁} {β : Type u₂} {γ : Type u₃}
+    (e : α ≃ β) (f : β ≃ γ) :
+    α ≃ γ where
+  toFun a := f.toFun (e.toFun a)
+  invFun c := e.invFun (f.invFun c)
+
+def Equiv.sumCongr {α₁ : Type u₁} {α₂ : Type u₂} {β₁ : Type u₃} {β₂ : Type u₄}
+    (ea : α₁ ≃ α₂) (eb : β₁ ≃ β₂) :
+    (α₁ ⊕ β₁) ≃ (α₂ ⊕ β₂) where
+  toFun := Sum.map ea.toFun eb.toFun
+  invFun := Sum.map ea.invFun eb.invFun
+
+def finSumFinEquiv {m n : Nat} :
+    (Fin m ⊕ Fin n) ≃ (Fin (m + n)) where
+  toFun := Sum.elim (Fin.castAdd n) (Fin.natAdd m)
+  invFun i := @Fin.addCases m n (fun _ => Fin m ⊕ Fin n) Sum.inl Sum.inr i
+  toFun_invFun i := by induction i using Fin.addCases <;> simp
