Db/Examples/Book.lean
@@ -1,0 +1,44 @@
+/-
+Copyright (c) 2025 Christian Merten. All rights reserved.
+Released under Apache 2.0 license as described in the file LICENSE.
+Authors: Christian Merten
+-/
+import Db
+
+namespace BookExample
+
+structure Author where
+  name : VarChar 100
+  age : Int
+  retired : Bool
+  deriving Repr
+
+generate_table BookExample.Author
+
+inductive Index where
+  | author
+  deriving DecidableEq, Hashable, Repr, Enum
+
+instance : ToString Index where
+  toString
+    | .author => "author"
+
+instance : FromString Index where
+  fromString
+    | "author" => some .author
+    | _ => none
+
+instance : Indexing Index where
+
+def database : Database where
+  Index := Index
+  tables
+    | .author => AuthorTable
+
+instance : HasTable Author (database.tables .author) :=
+  inferInstanceAs <| HasTable Author AuthorTable
+
+def authorModel : Model database Author where
+  index := .author
+
+end BookExample
