Db/Model.lean
@@ -1,0 +1,2 @@
+import Db.Model.HasTable
+import Db.Model.Meta
