Db/Model/HasTable.lean
@@ -1,0 +1,51 @@
+/-
+Copyright (c) 2025 Christian Merten. All rights reserved.
+Released under Apache 2.0 license as described in the file LICENSE.
+Authors: Christian Merten
+-/
+import Db.Query.Basic
+import Db.Utils.Equiv
+import Db.Interpretation.Basic
+
+/-- A type is associated with a database table if there
+is an equivalence with the entries of the table. -/
+class HasTable (α : Type) (t : Table) where
+  encoding : α ≃ t.Entry
+
+variable (α : Type) (t : Table) [HasTable α t]
+
+structure Model (d : Database) (α : Type) where
+  index : d.Index
+  [hasTable : HasTable α (d.tables index)]
+
+attribute [instance] Model.hasTable
+
+variable {d : Database} {α : Type} {model : Model d α}
+
+abbrev Model.table (model : Model d α) : Table :=
+  d.tables model.index
+
+-- TODO: add meta code / DSL (?) to construct querysets for models
+/-- A queryset for a model `m` is a query on the corresponding database table. -/
+def QuerySet {d : Database} {α : Type} (model : Model d α) : Type 1 :=
+  Query d (Table.names model.index)
+
+variable {m : Type → Type} [DBMonad d m] [Monad m] [MonadExcept String m]
+
+/-- Fetch the given queryset from the database. -/
+def QuerySet.fetch (q : QuerySet model) : m (Array α) := do
+  let res ← DBMonad.lookup q
+  res.filterMapM fun map => OptionT.run do
+    let x : model.table.Entry ← .mk <$> Enum.distribM fun c =>
+      let val := map.get? (.ident { tableName := model.index, columnName := c})
+      match val with
+      | some val => return val
+      | none =>
+        -- TODO: add logging here
+        failure
+    return HasTable.encoding.invFun x
+
+def Model.insert (model : Model d α) (a : α) : m Unit := do
+  let data : d.Insert model.index :=
+    { entry := HasTable.encoding.toFun a }
+  DBMonad.insert data
