Db/Utils/FinCases.lean
@@ -1,0 +1,42 @@
+import Lean
+
+/-
+Fin cases tactic, implementation inspired by mathlib's `fin_cases` tactic.
+-/
+
+open Lean Elab
+
+private def guardConcreteFin (expr : Expr) : MetaM Expr :=
+  match expr.getAppFnArgs with
+  | (``Fin, #[n]) => return n
+  | _ => throwError "Variable not of type `Fin ?n` for concrete `?n`."
+
+private def isMembership (expr : Expr) : Bool :=
+  match expr.getAppFnArgs with
+  | (``List.Mem, _) => true
+  | (``Membership.mem, _) => true
+  | _ => false
+
+partial def finCases (goal : MVarId) (var : FVarId) : MetaM (List MVarId) := goal.withContext do
+  let type ← var.getType >>= instantiateMVars
+  let _ ← guardConcreteFin type
+  let memListExpr ← Meta.mkAppM ``List.mem_finRange #[.fvar var]
+  let type ← Meta.inferType memListExpr
+  let (_, goal) ← (← goal.assert `this type memListExpr).intro1P
+  goal.casesRec fun decl => return isMembership decl.type
+
+elab "fincases" var:ident : tactic => do
+  let fvar ← Tactic.getFVarId var
+  Tactic.liftMetaTactic fun goal => finCases goal fvar
+
+section Tests
+
+def foobaz : Fin 3 → String
+  | 0 => "ho"
+  | 1 => "ho"
+  | 2 => "ho"
+
+example (i : Fin 3) : foobaz i = "ho" := by
+  fincases i <;> rfl
+
+end Tests
